vale/specs/interop/Interop.X64.fst
@@ -8,7 +8,7 @@ module TS = X64.Taint_Semantics_s
 module IA = Interop.Assumptions
 module ST = FStar.HyperStack.ST
 
-let wrap_variadic c down_mem num_b8_slots args #pre_rel #post_rel predict =
+let wrap_variadic c n arg_reg down_mem num_b8_slots args #pre_rel #post_rel predict =
   let h0 = ST.get () in
   let h0' = h0 in
   assert (mem_roots_p h0' args);
@@ -32,7 +32,7 @@ let wrap_variadic c down_mem num_b8_slots args #pre_rel #post_rel predict =
       (fun h0' -> h0' == alloc_push_h0)
       (fun h0' ->
         let va_s0, mem_s0 =
-          create_initial_trusted_state num_b8_slots args down_mem h0' stack_b in
+          create_initial_trusted_state n arg_reg num_b8_slots args down_mem h0' stack_b in
         let (rax, fuel, final_mem) = predict h0 va_s0 push_h0 alloc_push_h0 stack_b in
         assert (B.frameOf stack_b = HS.get_tip h0');
         assert (B.live h0' stack_b);
@@ -42,18 +42,20 @@ let wrap_variadic c down_mem num_b8_slots args #pre_rel #post_rel predict =
       ) in
   ST.pop_frame ();
   assert (ST.equal_domains alloc_push_h0 (hs_of_mem final_mem));
-  rax, Ghost.hide (As_lowstar_sig_ret num_b8_slots args push_h0 alloc_push_h0 stack_b fuel final_mem)
+  rax, Ghost.hide (As_lowstar_sig_ret n num_b8_slots args push_h0 alloc_push_h0 stack_b fuel final_mem)
 
 let rec wrap_aux
+    (n:nat)
+    (arg_reg:arg_reg_relation n)
     (down_mem:down_mem_t)
     (c:TS.tainted_code)
     (num_b8_slots:max_slots)
     (dom:list td)
-    (args:list arg{arity_ok_2 dom args})
-    (pre_rel:rel_gen_t c dom args (prediction_pre_rel_t c))
-    (post_rel:rel_gen_t c dom args (prediction_post_rel_t c num_b8_slots))
-    (predict:prediction_t down_mem c num_b8_slots dom args pre_rel post_rel)
-  : as_lowstar_sig_t down_mem c num_b8_slots dom args pre_rel post_rel predict
+    (args:list arg{arity_ok_2 n dom args})
+    (pre_rel:rel_gen_t n c dom args (prediction_pre_rel_t n c))
+    (post_rel:rel_gen_t n c dom args (prediction_post_rel_t n c num_b8_slots))
+    (predict:prediction_t n arg_reg down_mem c num_b8_slots dom args pre_rel post_rel)
+  : as_lowstar_sig_t n arg_reg down_mem c num_b8_slots dom args pre_rel post_rel predict
   = match dom with
     | [] ->
       let f () :
@@ -61,32 +63,34 @@ let rec wrap_aux
            (requires fun h0 ->
              mem_roots_p h0 args /\ elim_rel_gen_t_nil pre_rel h0)
            (ensures fun h0 ret h1 ->
-             as_lowstar_sig_post down_mem c num_b8_slots args h0 #pre_rel #post_rel (elim_predict_t_nil predict) ret h1) =
-        wrap_variadic c down_mem num_b8_slots args (elim_predict_t_nil predict)
+             as_lowstar_sig_post n arg_reg down_mem c num_b8_slots args h0 #pre_rel #post_rel (elim_predict_t_nil predict) ret h1) =
+        wrap_variadic c n arg_reg down_mem num_b8_slots args (elim_predict_t_nil predict)
       in
-      f <: as_lowstar_sig_t down_mem c num_b8_slots [] args pre_rel post_rel predict
+      f <: as_lowstar_sig_t n arg_reg down_mem c num_b8_slots [] args pre_rel post_rel predict
 
     | hd::tl ->
       fun (x:td_as_type hd) ->
-      wrap_aux down_mem c num_b8_slots tl
+      wrap_aux n arg_reg down_mem c num_b8_slots tl
         (x ++ args)
         (elim_rel_gen_t_cons hd tl pre_rel x)
         (elim_rel_gen_t_cons hd tl post_rel x)
         (elim_predict_t_cons hd tl predict x)
 
-let wrap down_mem c num_b8_slots dom #pre_rel #post_rel predict =
-  wrap_aux down_mem c num_b8_slots dom [] pre_rel post_rel predict
+let wrap n arg_reg down_mem c num_b8_slots dom #pre_rel #post_rel predict =
+  wrap_aux n arg_reg down_mem c num_b8_slots dom [] pre_rel post_rel predict
 
 let rec wrap_aux_weak
+    (n:nat)
+    (arg_reg:arg_reg_relation n)
     (down_mem:down_mem_t)
     (c:TS.tainted_code)
     (num_b8_slots:max_slots)
     (dom:list td)
-    (args:list arg{arity_ok_2 dom args})
-    (pre_rel:rel_gen_t c dom args (prediction_pre_rel_t c))
-    (post_rel:rel_gen_t c dom args (prediction_post_rel_t c num_b8_slots))
-    (predict:prediction_t down_mem c num_b8_slots dom args pre_rel post_rel)
-  : as_lowstar_sig_t_weak down_mem c num_b8_slots dom args pre_rel post_rel predict
+    (args:list arg{arity_ok_2 n dom args})
+    (pre_rel:rel_gen_t n c dom args (prediction_pre_rel_t n c))
+    (post_rel:rel_gen_t n c dom args (prediction_post_rel_t n c num_b8_slots))
+    (predict:prediction_t n arg_reg down_mem c num_b8_slots dom args pre_rel post_rel)
+  : as_lowstar_sig_t_weak n arg_reg down_mem c num_b8_slots dom args pre_rel post_rel predict
   = match dom with
     | [] ->
       let f () 
@@ -95,19 +99,20 @@ let rec wrap_aux_weak
              mem_roots_p h0 args /\ elim_rel_gen_t_nil pre_rel h0)
            (ensures fun h0 ret h1 ->
              as_lowstar_sig_post_weak
+               n arg_reg
                down_mem c num_b8_slots args h0 
                #pre_rel #post_rel (elim_predict_t_nil predict) ret h1)
-        = wrap_variadic c down_mem num_b8_slots args (elim_predict_t_nil predict)
+        = wrap_variadic c n arg_reg down_mem num_b8_slots args (elim_predict_t_nil predict)
       in
-      f <: as_lowstar_sig_t_weak down_mem c num_b8_slots [] args pre_rel post_rel predict
+      f <: as_lowstar_sig_t_weak n arg_reg down_mem c num_b8_slots [] args pre_rel post_rel predict
 
     | hd::tl ->
       fun (x:td_as_type hd) ->
-      wrap_aux_weak down_mem c num_b8_slots tl
+      wrap_aux_weak n arg_reg down_mem c num_b8_slots tl
         (x ++ args)
         (elim_rel_gen_t_cons hd tl pre_rel x)
         (elim_rel_gen_t_cons hd tl post_rel x)
         (elim_predict_t_cons hd tl predict x)
 
-let wrap_weak down_mem c num_b8_slots dom #pre_rel #post_rel predict =
-  wrap_aux_weak down_mem c num_b8_slots dom [] pre_rel post_rel predict
+let wrap_weak n arg_reg down_mem c num_b8_slots dom #pre_rel #post_rel predict =
+  wrap_aux_weak n arg_reg down_mem c num_b8_slots dom [] pre_rel post_rel predict
